Added optimized versions of [pack] and [unpack] to ModularBaseSystemOpt. Further optimization, including the unrolling of the entire loop, can be done in Specific/ once limb widths of both ModularBaseSystem format and wire format are known.

src/ModularArithmetic/ModularBaseSystemOpt.v
@@ -27,13 +27,19 @@ Class SubtractionCoefficient (m : Z) (prm : PseudoMersenneBaseParams m) := {
 
 (* Computed versions of some functions. *)
 
+Definition plus_opt := Eval compute in plus.
+
 Definition Z_add_opt := Eval compute in Z.add.
 Definition Z_sub_opt := Eval compute in Z.sub.
 Definition Z_mul_opt := Eval compute in Z.mul.
 Definition Z_div_opt := Eval compute in Z.div.
 Definition Z_pow_opt := Eval compute in Z.pow.
 Definition Z_opp_opt := Eval compute in Z.opp.
+Definition Z_min_opt := Eval compute in Z.min.
 Definition Z_ones_opt := Eval compute in Z.ones.
+Definition Z_of_nat_opt := Eval compute in Z.of_nat.
+Definition Z_le_dec_opt := Eval compute in Z_le_dec.
+Definition Z_lt_dec_opt := Eval compute in Z_lt_dec.
 Definition Z_shiftl_opt := Eval compute in Z.shiftl.
 Definition Z_shiftl_by_opt := Eval compute in Z.shiftl_by.
 
@@ -47,6 +53,10 @@ Definition base_from_limb_widths_opt := Eval compute in @Pow2Base.base_from_limb
 Definition minus_opt := Eval compute in minus.
 Definition max_ones_opt := Eval compute in @max_ones.
 Definition from_list_default_opt {A} := Eval compute in (@from_list_default A).
+Definition sum_firstn_opt {A} := Eval compute in (@sum_firstn A).
+Definition zeros_opt := Eval compute in (@zeros).
+Definition bit_index_opt := Eval compute in bit_index.
+Definition digit_index_opt := Eval compute in digit_index.
 
 Definition Let_In {A P} (x : A) (f : forall y : A, P y)
   := let y := x in f y.
@@ -407,7 +417,6 @@ Section Addition.
   Definition add_opt_sig (us vs : digits) : { b : digits | b = add us vs }.
   Proof.
     eexists.
-    cbv [BaseSystem.add].
     reflexivity.
   Defined.
 
@@ -621,6 +630,95 @@ Section Multiplication.
     carry_mul_opt_cps_correct id us vs.
 
 End Multiplication.
+
+Section Conversion.
+
+  Definition convert'_opt_sig {lwA lwB}
+             (nonnegA : forall x, In x lwA -> 0 <= x)
+             (nonnegB : forall x, In x lwB -> 0 <= x)
+             bits_fit inp i out :
+    { y | y = convert' nonnegA nonnegB bits_fit inp i out}.
+  Proof.
+    eexists.
+    rewrite convert'_equation.
+    change sum_firstn with @sum_firstn_opt.
+    change length with length_opt.
+    change Z_le_dec with Z_le_dec_opt.
+    change Z.of_nat with Z_of_nat_opt.
+    change digit_index with digit_index_opt.
+    change bit_index with bit_index_opt.
+    change Z.min with Z_min_opt.
+    change (nth_default 0 lwA) with (nth_default_opt 0 lwA).
+    change (nth_default 0 lwB) with (nth_default_opt 0 lwB).
+    cbv [update_by_concat_bits concat_bits Z.pow2_mod].
+    change Z.ones with Z_ones_opt.
+    change @update_nth with @update_nth_opt.
+    change plus with plus_opt.
+    change Z.sub with Z_sub_opt.
+    reflexivity.
+  Defined.
+
+  Definition convert'_opt {lwA lwB}
+             (nonnegA : forall x, In x lwA -> 0 <= x)
+             (nonnegB : forall x, In x lwB -> 0 <= x)
+             bits_fit inp i out := 
+    Eval cbv [proj1_sig convert'_opt_sig] in
+      proj1_sig (convert'_opt_sig nonnegA nonnegB bits_fit inp i out).
+
+  Definition convert'_opt_correct {lwA lwB}
+             (nonnegA : forall x, In x lwA -> 0 <= x)
+             (nonnegB : forall x, In x lwB -> 0 <= x)
+             bits_fit inp i out :
+    convert'_opt nonnegA nonnegB bits_fit inp i out = convert' nonnegA nonnegB bits_fit inp i out := 
+    Eval cbv [proj2_sig convert'_opt_sig] in
+      proj2_sig (convert'_opt_sig nonnegA nonnegB bits_fit inp i out).
+    
+  Context {modulus} (prm : PseudoMersenneBaseParams modulus)
+          {target_widths} (target_widths_nonneg : forall x, In x target_widths -> 0 <= x) (bits_eq : sum_firstn limb_widths (length limb_widths) = sum_firstn target_widths (length target_widths)).
+  Local Notation digits := (tuple Z (length limb_widths)).
+  Local Notation target_digits := (tuple Z (length target_widths)).
+
+  Definition pack_opt_sig (x : digits) : { y | y = pack target_widths_nonneg bits_eq x}.
+  Proof.
+    eexists.
+    cbv [pack].
+    rewrite <- from_list_default_eq with (d := 0%Z).
+    change @from_list_default with @from_list_default_opt.
+    cbv [ModularBaseSystemList.pack convert].
+    change length with length_opt.
+    change sum_firstn with @sum_firstn_opt.
+    change zeros with zeros_opt.
+    reflexivity.
+  Defined.
+
+  Definition pack_opt (x : digits) : target_digits :=
+    Eval cbv [proj1_sig pack_opt_sig] in proj1_sig (pack_opt_sig x).
+
+  Definition pack_correct (x : digits) :
+    pack_opt x = pack target_widths_nonneg bits_eq x
+    := Eval cbv [proj2_sig pack_opt_sig] in proj2_sig (pack_opt_sig x).
+
+  Definition unpack_opt_sig (x : target_digits) : { y | y = unpack target_widths_nonneg bits_eq x}.
+  Proof.
+    eexists.
+    cbv [unpack].
+    rewrite <- from_list_default_eq with (d := 0%Z).
+    change @from_list_default with @from_list_default_opt.
+    cbv [ModularBaseSystemList.unpack convert].
+    change length with length_opt.
+    change sum_firstn with @sum_firstn_opt.
+    change zeros with zeros_opt.
+    reflexivity.
+  Defined.
+
+  Definition unpack_opt (x : target_digits) : digits :=
+    Eval cbv [proj1_sig unpack_opt_sig] in proj1_sig (unpack_opt_sig x).
+  
+  Definition unpack_correct (x : target_digits) :
+    unpack_opt x = unpack target_widths_nonneg bits_eq x
+    := Eval cbv [proj2_sig unpack_opt_sig] in proj2_sig (unpack_opt_sig x).
+
+End Conversion.
 
 Section with_base.
   Context {modulus} (prm : PseudoMersenneBaseParams modulus).
